proof/correctness1024/Fq.ec
@@ -316,6 +316,29 @@ rewrite modz_dvd;  last by smt(W16.to_uint_cmp pow2_16).
 rewrite -pow2_4; apply dvdz_exp2l; smt().
 qed.
 
+lemma compress_impl5 (a : W16.t):
+  bpos16 a q =>
+  (to_uint (((zeroextu32 a `<<` W8.of_int 5) + 
+     W32.of_int 1664) * W32.of_int 40318 `>>` W8.of_int 27)) %% 32=
+       compress 5 (incoeff (to_sint a)).
+proof.
+have ? := pow2_5. 
+rewrite qE;move => abl; move : (to_sint_unsigned a _); 1: by smt().
+move => au; rewrite -compress_alt_compress5.
+rewrite /zeroextu32 /truncateu8 /compress_alt5 qE => /= *.
+rewrite  /(`<<`) /(`>>`) W32.shlMP; 1: by smt().
+rewrite W32.to_uint_shr; 1: by smt().
+rewrite incoeffK to_sintE /max /= !W32.of_uintK /= qE /=.
+rewrite !(modz_small _ 3329) /=; 1: smt().
+have ->: W16.smod (to_uint a) = to_uint a by
+  move : abl; rewrite /to_sint /smod /=; 1: by smt(W16.to_uint_cmp pow2_16).
+pose xx := (to_uint a * 32 + 1664).
+have -> : (4294967296 = 32*134217728) by auto. 
+rewrite divz_mod_mul 1..2://. 
+rewrite modz_dvd;  last by smt(W16.to_uint_cmp pow2_16).
+done.
+qed.
+
 
 lemma compress_impl_large (a : W16.t) :
   bpos16 a q =>
